Int encoder first if[wip] and loop[wip] [skip ci]

src/Primitive/Int/VstEnc.v
@@ -8,32 +8,235 @@ Definition Vprog : varspecs. Proof. mk_varspecs prog. Defined.
 
 Section Integer_der_encode.
 
+Definition prim_type_s := (Tstruct _ASN__PRIMITIVE_TYPE_s noattr).
+Definition mk_prim_type_s (buf_p : val) size := (buf_p, Vint (Int.repr size)).
+
+Definition int_enc_rval td li sptr_p := 
+  match evalErrW (int_encoder td li) [] with
+  | Some v => mk_enc_rval (encoded v) Vzero
+  | None => mk_enc_rval (-1) sptr_p
+  end.
+
+Definition int_enc_res td li := 
+  match execErrW (int_encoder td li) [] with
+  | Some v => v
+  | None => []
+  end.
+
 Definition int_der_encode_spec : ident * funspec :=
   DECLARE _INTEGER_encode_der
-    WITH res: val,  sptr_p : val, sptr_val : int, 
+    WITH res_p : val,  
+         sptr_p : val, buf_p : val, size : Z, data : list byte,
          td_p : val, td : TYPE_descriptor,
          tag_mode : Z, tag : Z,
          cb_p : val, app_key_p : val
     PRE [tptr enc_rval_s, tptr type_descriptor_s, tptr tvoid, tint, tuint, 
           tptr cb_type, tptr tvoid]
-      PROP (decoder_type td = BOOLEAN_t)
-      PARAMS (res; td_p; sptr_p; Vint (Int.repr tag_mode);
+      PROP (decoder_type td = BOOLEAN_t;
+            0 < size;
+            size = Zlength data;
+            (* if sptr_p is null, then encoder will crush *)
+            sptr_p <> nullval;
+            is_pointer_or_null buf_p)
+      PARAMS (res_p; td_p; sptr_p; Vint (Int.repr tag_mode);
               Vint (Int.repr tag); cb_p; app_key_p)
       GLOBALS ()
-      SEP ()
+      SEP (data_at_ Tsh enc_rval_s res_p;
+           data_at_ Tsh type_descriptor_s td_p; 
+           (* sptr *)
+           valid_pointer buf_p;
+           if Val.eq buf_p nullval 
+           then emp
+           else data_at Tsh (tarray tuchar size) (map Vbyte data) buf_p;
+           field_at Tsh prim_type_s (DOT _buf) buf_p sptr_p;
+           field_at Tsh prim_type_s (DOT _size) (Vint (Int.repr size)) sptr_p;
+           (* Callback *)
+           data_at_ Tsh enc_key_s app_key_p;
+           valid_pointer cb_p)
     POST [tvoid]
-      PROP()
+      PROP ()
       LOCAL ()
-      SEP().
+      SEP (data_at_ Tsh type_descriptor_s td_p;
+           (* sptr *)
+           valid_pointer buf_p;
+           if Val.eq buf_p nullval 
+           then emp
+           else data_at Tsh (tarray tuchar size) 
+                        (map Vbyte (int_enc_res td data)) buf_p;
+           data_at Tsh prim_type_s (mk_prim_type_s buf_p size) sptr_p;
+           (* Result *)
+           data_at Tsh enc_rval_s (int_enc_rval td data sptr_p) res_p;
+           (* Callback *)
+           valid_pointer cb_p;
+           data_at_ Tsh enc_key_s app_key_p;
+           func_ptr' dummy_callback_spec cb_p).
 
 Definition Gprog := ltac:(with_library prog [int_der_encode_spec]).
+
+Ltac forward_empty_loop :=
+      match goal with
+      | [ _ : _ |- semax _ ?Pre (Ssequence (Sloop Sskip Sbreak) _) _ ] =>
+          forward_loop Pre break: Pre; try forward ; try entailer! 
+      end. 
 
 Theorem int_der_encode : semax_body Vprog Gprog 
                                      (normalize_function f_INTEGER_encode_der
                                                          composites)
                                      int_der_encode_spec.
 Proof.
-  Fail start_function. 
+  start_function. 
+  rename H into DT; rename H0 into SgtZ; rename H1 into SeqDl.
+  replace (Tstruct _asn_enc_rval_s noattr) with enc_rval_s by reflexivity.
+  replace (Tstruct _ASN__PRIMITIVE_TYPE_s noattr) with prim_type_s by reflexivity.
+  forward.
+  forward_empty_loop.
+  forward_if (
+      PROP ( ) 
+      LOCAL (temp _t'2 buf_p; temp _st sptr_p; 
+             lvar __res__1 enc_rval_s v__res__1;
+             lvar _unconst (Tunion __3988 noattr) v_unconst;
+             lvar _effective_integer prim_type_s v_effective_integer;
+             lvar _rval (Tstruct _asn_enc_rval_s noattr) v_rval; 
+             temp __res res_p; temp _td td_p; 
+             temp _sptr sptr_p; temp _tag_mode (Vint (Int.repr tag_mode));
+             temp _tag (Vint (Int.repr tag)); 
+             temp _cb cb_p; temp _app_key app_key_p)
+       SEP ((* Local vars *)
+            data_at_ Tsh enc_rval_s v__res__1;
+            data_at_ Tsh (Tunion __3988 noattr) v_unconst;
+            data_at_ Tsh prim_type_s v_effective_integer;
+            data_at_ Tsh (Tstruct _asn_enc_rval_s noattr) v_rval; 
+            (* type descriptor *)
+            data_at_ Tsh type_descriptor_s td_p; 
+            (* sptr *)
+            valid_pointer buf_p;
+            if Val.eq buf_p nullval
+            then emp
+            else data_at Tsh (tarray tuchar size) (map Vbyte data) buf_p;
+            field_at Tsh prim_type_s (DOT _buf) buf_p sptr_p;
+            field_at Tsh prim_type_s (DOT _size) (Vint (Int.repr size)) sptr_p; 
+            (* Result *)
+            data_at_ Tsh enc_rval_s res_p;
+            (* Callback *)
+            data_at_ Tsh enc_key_s app_key_p;
+            valid_pointer cb_p)).
+  * (* st->buf <> null *)
+    destruct buf_p; try contradiction; rewrite if_false by discriminate.
+    repeat forward.
+    normalize.
+    forward_loop (EX z : Z, 
+               PROP ()
+               LOCAL (temp 
+                        _end1 
+                        (Vptr b 
+                              (Ptrofs.sub 
+                                 (Ptrofs.add i 
+                                             (Ptrofs.repr 
+                                                (Int.unsigned (Int.repr size)))) 
+                                 (Ptrofs.repr 1))); 
+                      temp _buf (Vptr b (Ptrofs.add i (Ptrofs.repr z))); 
+                      temp _t'10 (Vint (Int.repr size));
+                      temp _t'2 (Vptr b i); temp _st sptr_p;
+                      lvar __res__1 enc_rval_s v__res__1; 
+                      lvar _unconst (Tunion __3988 noattr) v_unconst;
+                      lvar _effective_integer prim_type_s v_effective_integer; 
+                      lvar _rval enc_rval_s v_rval; temp _tag (Vint (Int.repr tag));
+                      temp __res res_p; temp _td td_p; temp _sptr sptr_p;
+                      temp _tag_mode (Vint (Int.repr tag_mode));
+                      temp _cb cb_p; temp _app_key app_key_p)
+               SEP (data_at_ Tsh enc_rval_s v__res__1; 
+                    data_at_ Tsh (Tunion __3988 noattr) v_unconst;
+                    data_at_ Tsh prim_type_s v_effective_integer; 
+                    data_at_ Tsh enc_rval_s v_rval;
+                    data_at_ Tsh enc_rval_s res_p; data_at_ Tsh type_descriptor_s td_p;
+                    data_at_ Tsh enc_key_s app_key_p; valid_pointer (Vptr b i);
+                    data_at Tsh (tarray tuchar size) (map Vbyte data) (Vptr b i);
+                    field_at Tsh prim_type_s (DOT _buf) (Vptr b i) sptr_p;
+                    field_at Tsh prim_type_s (DOT _size) (Vint (Int.repr size)) sptr_p; 
+                    valid_pointer cb_p))%assert
+      continue: (EX z : Z, 
+               PROP ()
+               LOCAL (temp 
+                        _end1 
+                        (Vptr b 
+                              (Ptrofs.sub 
+                                 (Ptrofs.add i 
+                                             (Ptrofs.repr 
+                                                (Int.unsigned (Int.repr size)))) 
+                                 (Ptrofs.repr 1))); 
+                      temp _t'10 (Vint (Int.repr size));
+                      temp _buf (Vptr b (Ptrofs.add i (Ptrofs.repr z))); 
+                      temp _t'2 (Vptr b i); temp _st sptr_p;
+                      lvar __res__1 enc_rval_s v__res__1; 
+                      lvar _unconst (Tunion __3988 noattr) v_unconst;
+                      lvar _effective_integer prim_type_s v_effective_integer; 
+                      lvar _rval enc_rval_s v_rval; temp _tag (Vint (Int.repr tag));
+                      temp __res res_p; temp _td td_p; temp _sptr sptr_p;
+                      temp _tag_mode (Vint (Int.repr tag_mode));
+                      temp _cb cb_p; temp _app_key app_key_p)
+               SEP (data_at_ Tsh enc_rval_s v__res__1; 
+                    data_at_ Tsh (Tunion __3988 noattr) v_unconst;
+                    data_at_ Tsh prim_type_s v_effective_integer; 
+                    data_at_ Tsh enc_rval_s v_rval;
+                    data_at_ Tsh enc_rval_s res_p; data_at_ Tsh type_descriptor_s td_p;
+                    data_at_ Tsh enc_key_s app_key_p; valid_pointer (Vptr b i);
+                    data_at Tsh (tarray tuchar size) (map Vbyte data) (Vptr b i);
+                    field_at Tsh prim_type_s (DOT _buf) (Vptr b i) sptr_p;
+                    field_at Tsh prim_type_s (DOT _size) (Vint (Int.repr size)) sptr_p; 
+                    valid_pointer cb_p))%assert
+      break: (PROP ()
+              LOCAL (temp 
+                       _end1 
+                       (Vptr b 
+                             (Ptrofs.sub 
+                                (Ptrofs.add i 
+                                            (Ptrofs.repr 
+                                               (Int.unsigned (Int.repr size)))) 
+                                (Ptrofs.repr 1))); 
+                     temp _t'10 (Vint (Int.repr size));
+                     temp _buf (Vptr b i); temp _t'2 (Vptr b i); temp _st sptr_p;
+                     lvar __res__1 enc_rval_s v__res__1; 
+                     lvar _unconst (Tunion __3988 noattr) v_unconst;
+                     lvar _effective_integer prim_type_s v_effective_integer; 
+                     lvar _rval enc_rval_s v_rval; temp _tag (Vint (Int.repr tag));
+                     temp __res res_p; temp _td td_p; temp _sptr sptr_p;
+                     temp _tag_mode (Vint (Int.repr tag_mode));
+                     temp _cb cb_p; temp _app_key app_key_p)
+              SEP(data_at_ Tsh enc_rval_s v__res__1; 
+                  data_at_ Tsh (Tunion __3988 noattr) v_unconst;
+                  data_at_ Tsh prim_type_s v_effective_integer; 
+                  data_at_ Tsh enc_rval_s v_rval;
+                  data_at_ Tsh enc_rval_s res_p; data_at_ Tsh type_descriptor_s td_p;
+                  data_at_ Tsh enc_key_s app_key_p; valid_pointer (Vptr b i);
+                  data_at Tsh (tarray tuchar size) (map Vbyte data) (Vptr b i);
+                  field_at Tsh prim_type_s (DOT _buf) (Vptr b i) sptr_p;
+                  field_at Tsh prim_type_s (DOT _size) (Vint (Int.repr size)) sptr_p; 
+                  valid_pointer cb_p)).
+    - (* invariant check *)
+      Exists 0.
+      entailer!.
+    - (* loop *)
+      Intros z.
+      forward_if.
+      admit.
+      forward.
+Lemma split_array_head_tale : forall {cs : compspecs} size data p t,
+          size = Zlength data ->
+          data_at Tsh (tarray t size) data p = 
+          (data_at Tsh t (match hd_error data with
+                          | Some v => v
+                          | None => Vundef
+                          end) p) * 
+          (data_at Tsh (tarray t (size - 1)) (tl data) p)
+      rewrite split2_data_at_Tarray_app.
+      rewrite data_at_tuchar_singleton_array_eq.
+    - (* break postcondition check *)
+    
+  * (* postcondition check *)
+    forward.
+    entailer!.
+  * (* st->buf = null *)
+  
 Admitted.
 
 End Integer_der_encode.
